Lang/Simple.lean
@@ -1,0 +1,2 @@
+import Lang.Simple.Defs
+import Lang.Simple.Lift
